Prove the following
\begin{enumerate}
	\item If both $(A, \alpha, \gamma_1, C)$ and $(A, \alpha, \gamma_2, C)$ are Galois connections, then $\gamma_1 = \gamma_2$.
	\begin{proof}
		\begin{enumerate}
			\item From the definition of Galois connections we get:
			\begin{equation*}
			\alpha(c) \sqsubseteq a \iff c \sqsubseteq \gamma_1(a) \text{ and } \alpha(c) \sqsubseteq a \iff c \sqsubseteq \gamma_2(a) 
			\end{equation*}
			thus $c \sqsubseteq \gamma_1(a)\iff c \sqsubseteq \gamma_2(a)$.
			\item $\forall a \in A$ it holds that $\gamma_1(a) \sqsubseteq \gamma_1(a)$ and from the first step we get $\gamma_1(a) \sqsubseteq \gamma_2(a)$.
			\item Similarly $\forall a \in A$ it holds that $\gamma_2(a) \sqsubseteq \gamma_2(a)$ and from the first step we get $\gamma_2(a) \sqsubseteq \gamma_1(a)$.
			\item From the last 2 items we can construct:
			\begin{equation*}
			\forall a \in A: \qquad \gamma_1(a) \sqsubseteq \gamma_2(a) \sqsubseteq \gamma_1(a) \iff \gamma_1(a) = \gamma_2(a) \iff \gamma_1 = \gamma_2
			\end{equation*}
		\end{enumerate}
	\end{proof}
	\item If both $(A, \alpha_1, \gamma, C)$ and $(A, \alpha_2, \gamma, C)$ are Galois connections, then $\alpha_1 = \alpha_2$.
	\begin{proof}
		\begin{enumerate}
			\item From the definition of Galois connections we get:
			\begin{equation*}
				c \sqsubseteq \gamma(a) \iff \alpha_1(c)\sqsubseteq a \text{ and } c \sqsubseteq \gamma(a) \iff \alpha_2(c) \sqsubseteq a
			\end{equation*}
			thus $\alpha_1(c)\sqsubseteq a \iff \alpha_2(c) \sqsubseteq a$.
			\item $\forall c \in C$ it holds that $\alpha_1(c) \sqsubseteq \alpha_1(c)$ and from the first step we get $\alpha_1(c) \sqsubseteq \alpha_2(c)$.
			\item Similarly $\forall c \in C$ it holds that $\alpha_2(c) \sqsubseteq \alpha_2(c)$ and from the first step we get $\alpha_2(c) \sqsubseteq \alpha_1(c)$.
			\item From the last 2 items we can construct:
			\begin{equation*}
				\forall c \in C:\qquad \alpha_1(c) \sqsubseteq \alpha_2(c) \sqsubseteq \alpha_1(c) \iff \alpha_1(c) = \alpha_2(c) \iff \alpha_1 = \alpha_2
			\end{equation*}
		\end{enumerate}
	\end{proof}
\end{enumerate}